LogicalRefinement/Stlc/Interp.lean
@@ -127,33 +127,6 @@ theorem Term.stlc_ty_wknth {A: Term}: (A.wknth n).stlc_ty = A.stlc_ty
   apply Term.stlc_ty_wk
 }
 
-theorem Term.stlc_wknth_false {t: Term} {Γ: Sparsity} {n: Nat}
-: (t.wknth n).stlc (Γ.wknth n false) = t.stlc Γ
-:= by {
-  revert Γ n;
-  induction t with
-  | var v => 
-    intro Γ n;
-    simp only [wknth, wk]
-    repeat rw [stlc_var]
-    simp only [Sparsity.stlc, Sparsity.wknth_ix, Sparsity.wknth_dep]
-  | _ => 
-    intro Γ n;
-    simp only [wknth, wk]
-    repeat rw [Wk.lift_wknth_merge]
-    repeat rw [Wk.liftn_wknth_merge]
-    repeat rw [<-wknth_def] 
-    try (rename TermKind _ => k; cases k);
-    try (rename AnnotSort => s; cases s);
-    all_goals try rfl;
-    all_goals (
-      simp only [stlc] 
-      simp only [Sparsity.wknth_merge]
-      simp only [*]
-      repeat rw [Term.stlc_ty_wknth]
-    )
-}
-
 theorem Annot.stlc_ty_subst {Γ A σ s k} (H: Γ ⊢ A: sort s):
   (expr k (A.subst σ)).stlc_ty = (expr k A).stlc_ty := by {
     cases k with
