LogicalRefinement/Stlc/InterpWk.lean
@@ -1,0 +1,62 @@
+import LogicalRefinement.Untyped
+import LogicalRefinement.Typed
+import LogicalRefinement.Stlc.Basic
+import LogicalRefinement.Stlc.Interp
+import LogicalRefinement.Stlc.Subst
+
+set_option maxHeartbeats 1000000
+
+theorem Term.stlc_wknth_false {t: Term} {Γ: Sparsity} {n: Nat}
+: (t.wknth n).stlc (Γ.wknth n false) = t.stlc Γ
+:= by {
+  revert Γ n;
+  induction t with
+  | var v => 
+    intro Γ n;
+    simp only [wknth, wk]
+    repeat rw [stlc_var]
+    simp only [Sparsity.stlc, Sparsity.wknth_ix_false, Sparsity.wknth_dep]
+  | _ => 
+    intro Γ n;
+    simp only [wknth, wk]
+    repeat rw [Wk.lift_wknth_merge]
+    repeat rw [Wk.liftn_wknth_merge]
+    repeat rw [<-wknth_def] 
+    try (rename TermKind _ => k; cases k);
+    try (rename AnnotSort => s; cases s);
+    all_goals try rfl;
+    all_goals (
+      simp only [stlc] 
+      simp only [Sparsity.wknth_merge]
+      simp only [*]
+      repeat rw [Term.stlc_ty_wknth]
+    )
+}
+
+theorem Term.stlc_wknth_true {t: Term} {Γ: Sparsity} {n: Nat}
+: (t.wknth n).stlc (Γ.wknth n true) = (t.stlc Γ).wknth n
+:= by {
+  revert Γ n;
+  induction t;
+  case var v => 
+    intro Γ n;
+    simp only [wknth, wk]
+    repeat rw [stlc_var]
+    simp only [Sparsity.stlc, Sparsity.wknth_dep]
+    split
+    simp only [Stlc.wknth, Stlc.wk]
+    sorry
+    rfl
+    
+  all_goals (intro Γ n; simp only [wknth, wk, Stlc.wknth, Stlc.wk])
+
+  case natrec =>
+    simp only [stlc]
+    split
+    simp only [Sparsity.wknth_merge, Wk.liftn_wknth_merge, Wk.lift_wknth_merge]
+    simp only [<-wknth_def, *]
+    sorry
+    rfl
+
+  stop skip
+}
